src/program_proof/wal/installer_proof.v
@@ -1,0 +1,108 @@
+From RecordUpdate Require Import RecordSet.
+
+From Perennial.program_proof Require Import disk_lib.
+From Perennial.program_proof Require Import wal.invariant.
+
+Section goose_lang.
+Context `{!heapG Σ}.
+Context `{!lockG Σ}.
+Context `{!walG Σ}.
+
+Implicit Types (v:val) (z:Z).
+Implicit Types (γ: wal_names (Σ:=Σ)).
+Implicit Types (s: log_state.t) (memLog: list update.t) (txns: list (u64 * list update.t)).
+Implicit Types (pos: u64) (txn_id: nat).
+
+Context (P: log_state.t -> iProp Σ).
+Let N := walN.
+Let circN := walN .@ "circ".
+
+Definition in_bounds γ (a: u64): iProp Σ. Admitted.
+Instance in_bounds_persistent γ a : Persistent (in_bounds γ a).
+Proof. Admitted.
+
+(* TODO: this will actually require combining in_bounds with some authoritative
+resource from the invariant, obviously it can't be for an arbitrary [σ] *)
+Theorem in_bounds_valid γ σ a :
+  in_bounds γ a -∗ ⌜is_Some (σ.(log_state.d) !! int.val a)⌝.
+Proof. Admitted.
+
+(* this is more or less big_sepM_lookup_acc, but with is_installed_read unfolded *)
+Theorem is_installed_read_lookup {γ d txns installed_lb} {a: u64} :
+  is_Some (d !! int.val a) ->
+  is_installed_read γ d txns installed_lb -∗
+  ∃ txn_id b,
+    ⌜(installed_lb ≤ txn_id)%nat ∧
+      apply_upds (txn_upds (take txn_id txns)) d !! int.val a = Some b⌝ ∗
+    int.val a d↦ b ∗ (int.val a d↦ b -∗ is_installed_read γ d txns installed_lb).
+Proof.
+  rewrite /is_installed_read.
+  iIntros (Hlookup) "Hbs".
+  destruct Hlookup as [b0 Hlookup].
+  iDestruct (big_sepM_lookup_acc _ _ _ _ Hlookup with "Hbs") as "[Hb Hbs]".
+  iDestruct "Hb" as (b) "(%Hbvalue&Hb&%Ha_bound)".
+  destruct Hbvalue as [txn_id (Htxn_id_bound&Htxns_val)].
+  iExists txn_id, b.
+  iFrame "Hb".
+  iSplit; first by auto.
+  iIntros "Hb".
+  iApply ("Hbs" with "[Hb]").
+  { iExists _; iFrame.
+    iPureIntro; eauto. }
+Qed.
+
+(* simpler read_installed just for experimenting *)
+Definition log_read_installed (a:u64): transition log_state.t Block :=
+  installed_txn_id ← suchThat (fun s txn_id =>
+                                 s.(log_state.installed_lb) ≤
+                                 txn_id)%nat;
+  d ← reads (disk_at_txn_id installed_txn_id);
+  unwrap (d !! int.val a).
+
+Theorem wp_Walog__ReadInstalled (Q: Block -> iProp Σ) l γ a :
+  {{{ is_wal P l γ ∗
+      in_bounds γ a ∗
+       (∀ σ σ' b,
+         ⌜wal_wf σ⌝ -∗
+         ⌜relation.denote (log_read_installed a) σ σ' b⌝ -∗
+         (P σ ={⊤ ∖↑ N}=∗ P σ' ∗ Q b))
+   }}}
+    Walog__ReadInstalled #l #a
+  {{{ bl, RET slice_val bl; ∃ b, is_block bl b ∗ Q b}}}.
+Proof.
+  iIntros (Φ) "(#Hwal & #Ha_valid & Hfupd) HΦ".
+  wp_call.
+  wp_apply (wp_Read_fupd (⊤∖↑walN) (λ b, Q b)%I _ 1 (* q=1 *) with "[Hfupd]").
+  { iDestruct "Hwal" as "[Hwal Hcirc]".
+    iInv "Hwal" as (σ) "[Hinner HP]" "Hclose".
+    iDestruct "Hinner" as "(>? & ? & >? & ? & Hinstalled & ?)"; iNamed.
+    iDestruct (is_installed_to_read with "Hinstalled") as "[>Hinstalled_read Hinstalled]".
+    iDestruct (in_bounds_valid _ σ with "Ha_valid") as %Hlookup.
+    iDestruct (is_installed_read_lookup Hlookup with "Hinstalled_read") as
+        (txn_id b [Htxn_id Hbval]) "(Hb&Hinstalled_read)".
+    iModIntro.
+    iExists b; iFrame "Hb".
+    iNext.
+    iIntros "Hb".
+    iSpecialize ("Hinstalled_read" with "Hb").
+    iSpecialize ("Hinstalled" with "Hinstalled_read").
+    iMod ("Hfupd" $! σ σ b with "[//] [] HP") as "[HP HQ]".
+    { iPureIntro.
+      repeat (simpl; monad_simpl).
+      exists σ txn_id.
+      { econstructor; eauto. }
+      repeat (simpl; monad_simpl). }
+    iFrame.
+    iApply "Hclose".
+    iModIntro.
+    iExists _; iFrame "HP".
+    iFrame.
+    auto.
+  }
+  iIntros (s b) "(HQ&Hs)".
+  iApply "HΦ".
+  iExists _; iFrame.
+  iDestruct (is_slice_to_small with "Hs") as "$".
+Qed.
+
+End goose_lang.
